

A Numerical Approach to Computing $\mathcal{R}_c(t)$

Todd

January 26, 2026

We need to compute

$$p(t) = \mathbb{P} \{ \text{an individual infected at time } t \text{ infects a neighbour} \}. \quad (1)$$

The primary will infect the secondary if it makes an infectious contact before recovering *and* the secondary is not infected at the time of contact. Using the MSV formalism, the probability that a randomly chosen neighbour is not infected at time t is $\sigma(t) = G_q(\phi(t))$.

One way to compute $p(t)$ is by comparing times of random events: let T_r be the time after infection that the primary recovers, T_c be the time after infection that the primary makes its first contact with the secondary, and let T_n be the first time that the secondary neighbour has an infectious contact from one of its other neighbours:

$$\mathbb{P} \{ T_r > u \} = e^{-\gamma u} \quad (2a)$$

$$\mathbb{P} \{ T_c > u \} = e^{-\beta u} \quad (2b)$$

$$\mathbb{P} \{ T_n > t + u \} = \sigma(t + u). \quad (2c)$$

Further,

$$p(t) = \mathbb{P} \{ t + T_c < (t + T_r) \wedge T_n \}, \quad (3)$$

where \wedge denotes the minimum (this notation is commonly used in probability and stochastic processes), while, exploiting the independence of T_r and T_n ,

$$\mathbb{P} \{ (t + T_r) \wedge T_n > t + u \} = \mathbb{P} \{ T_r > u; T_n > t + u \} \quad (4a)$$

$$= \mathbb{P} \{ T_r > u \} \mathbb{P} \{ T_n > t + u \} \quad (4b)$$

$$= e^{-\gamma u} \sigma(t + u). \quad (4c)$$

Thus,

$$p(t) = \int_0^\infty \beta e^{-(\beta+\gamma)u} \sigma(t + u) du \quad (5)$$

and

$$\frac{dp}{dt} = \int_0^\infty \beta e^{-(\beta+\gamma)u} \frac{d}{dt} \sigma(t + u) du \quad (6a)$$

$$= \int_0^\infty \beta e^{-(\beta+\gamma)u} \frac{d}{du} \sigma(t + u) du \quad (6b)$$

$$= \beta e^{-(\beta+\gamma)u} \sigma(t + u) \Big|_0^\infty + \int_0^\infty \beta(\beta + \gamma) e^{-(\beta+\gamma)u} \sigma(t + u) du \quad (6c)$$

$$= (\beta + \gamma)p(t) - \beta\sigma(t). \quad (6d)$$

We can thus add one additional equation to the MSV equations to compute $p(t)$.

What is missing here are boundary conditions. Now, if we look at (5), $\sigma(t+u)$ is bounded, while $e^{-(\beta+\gamma)u}$ is integrable, so we can use Lebesgue's dominated convergence theorem to interchange integration and limits to see that

$$\lim_{t \rightarrow \infty} p(t) = \int_0^\infty \beta e^{-(\beta+\gamma)u} \lim_{t \rightarrow \infty} \sigma(t+u) du \quad (7a)$$

$$= \int_0^\infty \beta e^{-(\beta+\gamma)u} G_q(\phi(\infty)) du \quad (7b)$$

$$= \frac{\beta}{\beta+\gamma} G_q(\phi(\infty)). \quad (7c)$$

This is the final condition that allows us to compute $p(t)$; one way to do so is via the *shooting method*: we look for the value $p(0) = p_0$ so that the solution with this initial condition eventually goes to the correct final condition.

We can also approximate the initial condition by linearizing $\ell = -\ln \phi$ about the disease-free equilibrium, taking $\ell(0) = \ell_0$ where $0 < \ell_0 \ll 1$. We then have

$$-\dot{\ell} = -\beta + \beta G_q(e^{-\ell})e^\ell + \gamma(1 - e^\ell) \quad (8a)$$

$$= -\beta + \beta \frac{\sum_{d=1}^\infty dp_d e^{-(d-1)\ell}}{\sum_{d=1}^\infty dp_d} + \gamma(1 - e^\ell) \quad (8b)$$

$$= -\left(\beta \frac{\sum_{d=1}^\infty d(d-1)p_d}{\sum_{d=1}^\infty dp_d} + \gamma \right) \ell + \mathcal{O}(\ell^2) \quad (8c)$$

$$= -(\beta G'_q(1) + \gamma) \ell + \mathcal{O}(\ell^2) \quad (8d)$$

whence, keeping only the lowest order terms,

$$\ell(t) = \ell_0 e^{(\beta G'_q(1) + \gamma)t}. \quad (9)$$

Substituting $\phi(t) = e^{-\ell(t)}$ into (5) using (9) yields

$$p(0) = \int_0^\infty \beta e^{-(\beta+\gamma)t} G_q(e^{-\ell_0 e^{(\beta G'_q(1) + \gamma)t}}) dt. \quad (10a)$$

making the change of variable $u = \ell_0 e^{(\beta G'_q(1) + \gamma)t}$, we have

$$= \frac{\beta}{\beta G'_q(1) + \gamma} \ell_0^{\frac{\beta+\gamma}{\beta G'_q(1) + \gamma}} \int_{\ell_0}^\infty u^{-\frac{\beta+\gamma}{\beta G'_q(1) + \gamma} - 1} G_q(e^{-u}) du. \quad (10b)$$

Now, let's make a few observations. First, since $G_q(z)$ is a generating function, it is increasing, and has an increasing derivative. Moreover, $G_q(0) = 0$, as by definition, it is the p.g.f. of the degree of a vertex with at least one neighbour. Thus, using the mean value theorem, for any $z \in (0, 1)$ there exists $\eta \in [0, z]$ such that

$$\frac{G_q(z)}{z} = G'_q(\zeta), \quad (11)$$

so that $G'_q(0)z \leq G_q(z) \leq G'_q(1)z$. Thus,

$$\begin{aligned} G'_q(0) \int_{\ell_0}^{\infty} u^{-\frac{\beta+\gamma}{\beta G'_q(1)+\gamma}-1} e^{-u} du \\ \leq \int_{\ell_0}^{\infty} u^{-\frac{\beta+\gamma}{\beta G'_q(1)+\gamma}-1} G_q(e^{-u}) du \leq G'_q(1) \int_{\ell_0}^{\infty} u^{-\frac{\beta+\gamma}{\beta G'_q(1)+\gamma}-1} e^{-u} du, \end{aligned} \quad (12)$$

and the left and right hand side limits exist as $\ell_0 \rightarrow 0$:

$$\int_0^{\infty} u^{-\frac{\beta+\gamma}{\beta G'_q(1)+\gamma}-1} e^{-u} du = \Gamma\left(-\frac{\beta+\gamma}{\beta G'_q(1)+\gamma}\right), \quad (13)$$

which is well posed because $0 < \frac{\beta+\gamma}{\beta G'_q(1)+\gamma} < 1$ (recall that $\mathcal{R}_{0,c} = \frac{\beta}{\beta+\gamma G'_q(1)} \geq 1$). Moreover, all integrands in (12) are positive, and are thus all the integrals are increasing functions of ℓ_0 , so the integral

$$\int_0^{\infty} u^{-\frac{\beta+\gamma}{\beta G'_q(1)+\gamma}-1} G_q(e^{-u}) du \quad (14)$$

exists, and is bounded and non-zero.

Next, using l'Hôpital's rule, we see that

$$\lim_{\ell_0 \rightarrow 0} \frac{\int_0^{\infty} u^{-\frac{\beta+\gamma}{\beta G'_q(1)+\gamma}-1} G_q(e^{-u}) du - \int_{\ell_0}^{\infty} u^{-\frac{\beta+\gamma}{\beta G'_q(1)+\gamma}-1} G_q(e^{-u}) du}{\ell_0^{-\frac{\beta+\gamma}{\beta G'_q(1)+\gamma}}} \quad (15a)$$

$$= \lim_{\ell_0 \rightarrow 0} \frac{\int_0^{\ell_0} u^{-\frac{\beta+\gamma}{\beta G'_q(1)+\gamma}-1} G_q(e^{-u}) du}{\ell_0^{-\frac{\beta+\gamma}{\beta G'_q(1)+\gamma}}} \quad (15b)$$

$$= \lim_{\ell_0 \rightarrow 0} \frac{\ell_0^{-\frac{\beta+\gamma}{\beta G'_q(1)+\gamma}-1} G_q(e^{-\ell_0})}{-\frac{\beta+\gamma}{\beta G'_q(1)+\gamma} \ell_0^{-\frac{\beta+\gamma}{\beta G'_q(1)+\gamma}-1}} \quad (15c)$$

$$= -\frac{\beta G'_q(1) + \gamma}{\beta + \gamma}. \quad (15d)$$

Combining the above, we see that

$$\begin{aligned} \int_{\ell_0}^{\infty} u^{-\frac{\beta+\gamma}{\beta G'_q(1)+\gamma}-1} G_q(e^{-u}) du \\ = \int_0^{\infty} u^{-\frac{\beta+\gamma}{\beta G'_q(1)+\gamma}-1} G_q(e^{-u}) du - \ell_0^{-\frac{\beta+\gamma}{\beta G'_q(1)+\gamma}} \left(\frac{\beta G'_q(1) + \gamma}{\beta + \gamma} + o(\ell_0) \right). \end{aligned} \quad (16)$$

Substituting this into (10b) gives us

$$p(0) = \frac{\beta}{\beta + \gamma} + \frac{\beta}{\beta G'_q(1) + \gamma} \ell_0^{\frac{\beta+\gamma}{\beta G'_q(1)+\gamma}} \int_0^{\infty} u^{-\frac{\beta+\gamma}{\beta G'_q(1)+\gamma}-1} G_q(e^{-u}) du + o(\ell_0). \quad (17)$$

Now, we've already observed that $\frac{\beta+\gamma}{\beta G'_q(1)+\gamma} = \frac{1}{\mathcal{R}_{0,c} + \frac{\gamma}{\beta+\gamma}}$ lies strictly in $(0,1)$, so the initial condition ℓ_0 is appearing in a form that is strictly larger than $\mathcal{O}(\ell_0)$, with the effect becoming more pronounced as $\mathcal{R}_{0,c}$ increases.

The missing step here is to characterize ℓ_0 . Given that $S(t) = G_p(\phi(t))$ we might reasonably take $S(0) = 1 - \frac{1}{n}$ and $\phi(0) = G_p^{-1}(1 - \frac{1}{n})$, whence, using the inverse function theorem,

$$\ell_0 = -\ln G_p^{-1}\left(1 - \frac{1}{n}\right) \approx -\ln\left(1 - \frac{(G_p^{-1})'(1)}{n}\right) = -\ln\left(1 - \frac{1}{G'_p(1)n}\right) \approx \frac{1}{G'_p(1)n}, \quad (18)$$

and $p(0) - \frac{\beta}{\beta+\gamma} = \mathcal{O}\left(n^{-\frac{1}{\mathcal{R}_{0,c} + \frac{\gamma}{\beta+\gamma}}}\right)$.